Is0/Programs.lean
@@ -4,12 +4,15 @@ import Mathlib.Data.Vector
 import Mathlib.Data.ZMod.Defs
 import Mathlib.Data.ZMod.Basic
 import Mathlib.Tactic.LibrarySearch
+import Mathlib.Tactic.FieldSimp
 
 import Is0.Basic
 import Is0.Ending
 import Is0.Lemmas
 
 namespace Risc0
+
+open MLIRNotation
 
 open MLIRNotation in
 def is0_witness (input : List Felt) : List Felt :=
@@ -22,10 +25,23 @@ def is0_witness (input : List Felt) : List Felt :=
              } <|
     "x"         ←ₐ input[0];
     "isZeroBit" ←ₐ ??₀⟨"x"⟩;
-    output[0]   ←ₐ ⟨"isZeroBit"⟩;
+    output[0]   ←ᵢ ⟨"isZeroBit"⟩;
     "invVal"    ←ₐ Inv ⟨"x"⟩;
-    output[1]   ←ₐ ⟨"invVal"⟩
+    output[1]   ←ᵢ ⟨"invVal"⟩
   state'.output
+
+    -- %0 = cirgen.const 1
+    -- %1 = cirgen.true
+    -- %2 = cirgen.get %arg0[0] back 0 : <1, constant>
+    -- %3 = cirgen.get %arg1[0] back 0 : <2, mutable>
+    -- %4 = cirgen.and_eqz %1, %2 : <default>
+    -- %5 = cirgen.and_cond %1, %3 : <default>, %4
+    -- %6 = cirgen.sub %0 : <default>, %3 : <default>
+    -- %7 = cirgen.get %arg1[1] back 0 : <2, mutable>
+    -- %8 = cirgen.mul %2 : <default>, %7 : <default>
+    -- %9 = cirgen.sub %8 : <default>, %0 : <default>
+    -- %10 = cirgen.and_eqz %1, %9 : <default>
+    -- %11 = cirgen.and_cond %5, %6 : <default>, %10
 
 open MLIRNotation in
 def is0_constraints (input : List Felt) (output : List Felt) : Prop :=
@@ -36,104 +52,153 @@ def is0_constraints (input : List Felt) (output : List Felt) : Prop :=
              , output := output
              , constraints := []
              } <|
-    "1"         ←ₐ 1;
-    "x"         ←ₐ input[0];
-    "out[0]"    ←ₐ output[0];
-    guard ⟨"out[0]"⟩ then
-      ?₀⟨"x"⟩;
-    "1 - out[0]" ←ₐ ⟨"1"⟩ - ⟨"out[0]"⟩;
-    guard ⟨"1 - out[0]"⟩ then (
-      "out[1]"         ←ₐ output[1];
-      "x * out[1]"     ←ₐ ⟨"x"⟩ * ⟨"out[1]"⟩;
-      "x * out[1] - 1" ←ₐ ⟨"x * out[1]"⟩ - ⟨"1"⟩;
-      ?₀ ⟨"x * out[1] - 1"⟩
-    )
-  (List.foldr And True) $ List.map (λ e ↦ e = 0) state'.constraints
+    "1"         ←ₐ C 1;         -- %0 = cirgen.const 1
+    "0"         ←ₐ C 0;
+    "true"      ←ₐ ⊤;  -- %1 = cirgen.true
+    "x"         ←ₐ input[0];  -- %2 = cirgen.get %arg0[0] back 0 : <1, constant>
+    "out[0]"    ←ₐ output[0]; -- %3 = cirgen.get %arg1[0] back 0 : <2, mutable>
+    "andEqz x"  ←ₐ ⟨"true"⟩ &₀ ⟨"x"⟩; -- %4 = cirgen.and_eqz %1, %2 : <default>
+    "if out[0] then eqz x" ←ₐ guard ⟨"out[0]"⟩ & ⟨"true"⟩ with ⟨"andEqz x"⟩;  -- %5 = cirgen.and_cond %1, %3 : <default>, %4
+    "1 - out[0]" ←ₐ ⟨"1"⟩ - ⟨"out[0]"⟩; -- %6 = cirgen.sub %0 : <default>, %3 : <default>
+    "out[1]"         ←ₐ output[1]; -- %7 = cirgen.get %arg1[1] back 0 : <2, mutable>
+    "x * out[1]"     ←ₐ ⟨"x"⟩ * ⟨"out[1]"⟩; -- %8 = cirgen.mul %2 : <default>, %7 : <default>
+    "x * out[1] - 1" ←ₐ ⟨"x * out[1]"⟩ - ⟨"1"⟩; -- %9 = cirgen.sub %8 : <default>, %0 : <default>
+    "other cond" ←ₐ ⟨"true"⟩ &₀ ⟨"x * out[1] - 1"⟩; -- %10 = cirgen.and_eqz %1, %9 : <default>
+    "if other cond" ←ₐ guard ⟨"1 - out[0]"⟩ & ⟨"if out[0] then eqz x"⟩ with ⟨"other cond"⟩ -- %11 = cirgen.and_cond %5, %6 : <default>, %10
+  -- (List.foldr And True) $ List.map (λ e ↦ e = 0) state'.constraints
+  (state'.props "if other cond").getD True
 
+open MLIR in
 theorem is0_original_nondet_iff_constraints
   {input output : List Felt}
   (h : input.length = 1 ∧ output.length = 2) :
   (is0_witness input = output ↔ is0_constraints input output) := by
+  unfold is0_constraints
   rcases h with ⟨hin, hout⟩
   rcases input with _ | ⟨x, _ | _⟩ <;> simp at hin ; clear hin
   rcases output with _ | ⟨y₁, _ | ⟨y₂, ⟨_ | _⟩⟩⟩ <;> simp at hout ; clear hout
-  unfold is0_witness
+  -- unfold is0_witness
   rw [MLIR.run_Sequence_Assign_collapsible]
   simp only [Op.eval_getInput, List.getD_cons_zero, State.update_val]
   rw [MLIR.run_Sequence_Assign_collapsible]
+  simp only [Op.eval_const, State.update_val]
+  rw [MLIR.run_Sequence_Assign_collapsible]
   simp only [Op.eval_isz, Map.update_get, beq_iff_eq, ite_true, State.update_val]
-  rw [MLIR.run_Sequence_Set_collapsible (if x = 0 then 1 else 0) (by simp only [Map.update_get])] ; simp only
-  rw [MLIR.run_Sequence_Assign_collapsible]
-  simp only [Op.eval_inv, beq_iff_eq, State.update_val]
-  rw [Map.update_update_get (by decide)]
-  simp only [inv_zero, ite_self]
-  rw [@run_setOutput_of_some _ 1 (if x = 0 then 0 else x⁻¹) _ (by simp only [Map.update_get])] ; simp only
-  unfold List.set List.set ; simp only [List.cons.injEq, and_true]
-  unfold is0_constraints
-  rw [MLIR.run_Sequence_Assign_collapsible]
-  simp only [Op.eval_const_one, State.update_val]
   rw [MLIR.run_Sequence_Assign_collapsible]
   simp only [Op.eval_getInput, List.getD_cons_zero, State.update_val]
   rw [MLIR.run_Sequence_Assign_collapsible]
   simp only [Op.eval_getOutput, List.getD_cons_zero, State.update_val]
-  rw [MLIR.run_Sequence_If_collapsible y₁ (by simp only [Map.update_get])]
-  simp only [beq_iff_eq]
+  rw [MLIR.run_Sequence_Assign_collapsible]
+  simp
+  rw [Map.update_update_get (by decide)]
+  simp only [Option.some.injEq, forall_apply_eq_imp_iff', Op.eval.match_2.eq_2]
+  rw [MLIR.run_Sequence_Assign_collapsible]
+  simp only [
+    Op.eval_andCond, Map.update_get, beq_iff_eq, Option.some.injEq, eq_iff_iff, true_iff,
+    State.update_constraint]
+  rw [Map.update_update_get (by decide)]
+  simp only [true_and]
   rw [MLIR.run_Sequence_Assign_collapsible]
   simp only [Op.eval_sub, Map.update_get, Option.some.injEq, forall_apply_eq_imp_iff', State.update_val]
-  rw [@Map.update_get' _ _ _ _ "1" "out[0]" 1 _ (by simp) _]
+  rw [Map.update_get' 1 (by simp) _]
   swap
-  rw [Map.update_update_get (by simp)]
+  rw [Map.update_get' 1] <;> decide
   simp only
-  rw [MLIR.run_If_collapsible (1 - y₁) (by simp)]
-  simp only [beq_iff_eq]
   rw [MLIR.run_Sequence_Assign_collapsible]
   simp only [Op.eval_getOutput, List.getD_cons_succ, List.getD_cons_zero, State.update_val]
   rw [MLIR.run_Sequence_Assign_collapsible]
   simp only [Op.eval_mul, Map.update_get, Option.some.injEq, forall_apply_eq_imp_iff', State.update_val]
-  rw [@Map.update_get' _ _ _ _ "x" "out[1]" x _ (by simp) _] ; simp only
+  rw [Map.update_get' x] <;> try decide
   swap
-  rw [@Map.update_get' _ _ _ _ "x" "1 - out[0]" x _ (by simp) _] ; simp only
-  rw [@Map.update_get' _ _ _ _ "x" "out[0]" x _ (by simp) _] ; simp only
-  simp only [Map.update_get]
-  rw [MLIR.run_Sequence_Assign_collapsible]
-  simp only [Op.eval_sub, Map.update_get, Option.some.injEq, State.update_val]
-  rw [@Map.update_get' _ _ _ _ "1" "x * out[1]" 1 _ (by simp) _] ; simp only
-  swap
-  rw [@Map.update_get' _ _ _ _ "1" "out[1]" 1 _ (by simp) _] ; simp only
-  rw [@Map.update_get' _ _ _ _ "1" "1 - out[0]" 1 _ (by simp) _] ; simp only
-  rw [@Map.update_get' _ _ _ _ "1" "out[0]" 1 _ (by simp) _] ; simp only
-  rw [@Map.update_get' _ _ _ _ "1" "x" 1 _ (by simp) _] ; simp only
-  rw [@run_Eqz_of_some _ (x * y₂ - 1) _ (by simp)] ; simp only
-  rw [MLIR.run_Sequence_Eqz_collapsible x]
-  swap
-  simp only
-  rw [Map.update_update_get (by simp)]
+  rw [Map.update_get' x] <;> try decide
+  rw [Map.update_update_get (by decide)]
   simp only
   rw [MLIR.run_Sequence_Assign_collapsible]
-  simp only [Op.eval_sub, Map.update_get, Option.some.injEq, forall_apply_eq_imp_iff', State.update_val]
-  rw [@Map.update_get' _ _ _ _ "1" "out[0]" 1 _ (by simp) (by rw [Map.update_update_get (by simp)])] ; simp only
-  rw [MLIR.run_If_collapsible (1 - y₁) (by simp)]
-  simp only [beq_iff_eq]
-  rw [MLIR.run_Sequence_Assign_collapsible]
-  simp only [Op.eval_getOutput, List.getD_cons_succ, List.getD_cons_zero, State.update_val]
-  rw [MLIR.run_Sequence_Assign_collapsible]
-  simp only [Op.eval_mul, Map.update_get, Option.some.injEq, forall_apply_eq_imp_iff', State.update_val]
-  rw [@Map.update_get' _ _ _ _ "x" _ x _ (by simp) _] ; simp only
-  swap
-  rw [@Map.update_get' _ _ _ _ "x" _ x _ (by simp) _] ; simp only
-  rw [@Map.update_get' _ _ _ _ "x" _ x _ (by simp) _] ; simp only
-  simp only [Map.update_get]
-  rw [MLIR.run_Sequence_Assign_collapsible]
   simp only [Op.eval_sub, Map.update_get, Option.some.injEq, State.update_val]
-  rw [@Map.update_get' _ _ _ _ "1" _ 1 _ (by simp) _] ; simp only
+  rw [Map.update_get' 1] <;> try decide
   swap
-  rw [@Map.update_get' _ _ _ _ "1" _ 1 _ (by simp) _] ; simp only
-  rw [@Map.update_get' _ _ _ _ "1" _ 1 _ (by simp) _] ; simp only
-  rw [@Map.update_get' _ _ _ _ "1" _ 1 _ (by simp) _] ; simp only
-  rw [@Map.update_get' _ _ _ _ "1" _ 1 _ (by simp) _] ; simp only
-  rw [@run_Eqz_of_some _ (x * y₂ - 1) _ (by simp)] ; simp only
-  rw [State.if_constraints]
-  simp only [State.if_constraints]
-  apply ending
-
+  rw [Map.update_get' 1] <;> try decide
+  rw [Map.update_get' 1] <;> try decide
+  rw [Map.update_get' 1] <;> try decide
+  rw [Map.update_get' 1] <;> try decide
+  simp
+  rw [MLIR.run_Sequence_Assign_collapsible]
+  simp only [Op.eval_andEqz, Map.update_get, Option.some.injEq, forall_apply_eq_imp_iff',
+  State.update_constraint]
+  rw [Map.update_get' True] <;> try decide
+  swap
+  rw [Map.update_update_get (by decide)]
+  simp only [true_and]
+  rw [MLIR.run_assign]
+  simp only [Op.eval_andCond, Map.update_get, beq_iff_eq, Option.some.injEq, eq_iff_iff,
+  State.update_constraint, Option.getD_some]
+  rw [Map.update_get' (Sub.sub 1 y₁)] <;> try decide
+  swap
+  rw [Map.update_get' (Sub.sub 1 y₁)] <;> try decide
+  rw [Map.update_get' (Sub.sub 1 y₁)] <;> try decide
+  simp
+  rfl
+  rw [Map.update_get' (if y₁ = 0 then True else x = 0)] <;> try decide
+  swap
+  simp
+  simp
+  generalize h :
+    (if Sub.sub 1 y₁ = 0 then
+      if y₁ = 0 then True else x = 0
+        else (if y₁ = 0 then True else x = 0) ∧ HSub.hSub (HMul.hMul x y₂) 1 = 0) = finalCond
+  unfold is0_witness
+  rw [MLIR.run_Sequence_Assign_collapsible]
+  simp only [Op.eval_getInput, List.getD_cons_zero, State.update_val]
+  rw [MLIR.run_Sequence_Assign_collapsible]
+  simp only [Op.eval_isz, Map.update_get, beq_iff_eq, State.update_val]
+  rw [MLIR.run_Sequence_Set_collapsible (if x = 0 then 1 else 0)]
+  swap
+  simp
+  simp only
+  rw [MLIR.run_Sequence_Assign_collapsible]
+  simp only [Op.eval_inv, beq_iff_eq, State.update_val]
+  rw [Map.update_update_get (by decide)]
+  simp only
+  rw [MLIR.run_set]
+  simp only [Map.update_get]
+  apply Iff.intro
+  · intros h₁
+    subst h
+    by_cases eq : x = 0 <;> simp [eq]
+    · by_cases eq₁ : y₁ = 0 <;> simp [eq₁]
+      subst eq₁
+      subst eq
+      simp at h₁
+      simp [List.set] at h₁
+      subst eq
+      simp at h₁
+      simp [List.set] at h₁
+      rcases h₁ with ⟨h₁, h₂⟩
+      subst h₁
+      subst h₂
+      simp
+    · by_cases eq₁ : y₁ = 0 <;> simp [eq₁]
+      · subst eq₁
+        simp [List.set] at h₁
+        rw [←h₁.2]
+        simp [eq]
+      · simp [eq, eq₁, List.set] at h₁
+        tauto
+  -- Other directioon
+  have kekW : x ≠ 0 := sorry
+  subst h
+  intros h
+  simp [kekW]
+  by_cases eq : y₁ = 0 <;> simp [eq] at *
+  · simp at h
+    simp [List.set]
+    field_simp [h]
+    rw [←add_left_inj 1] at h
+    simp at h
+    rw [←h]
+    ring
+  · simp [List.set] at h
+    field_simp [h]
+    simp [List.set]
+    by_cases eq₁ : y₁ = 0 <;> simp [*] at *
 end Risc0
